IsaSAT: use definition for trail relation

Weidenbach_Book/IsaSAT_Trail_LLVM.thy
@@ -1,5 +1,5 @@
 theory IsaSAT_Trail_LLVM
-imports IsaSAT_Literals_LLVM IsaSAT_Trail   
+imports IsaSAT_Literals_LLVM IsaSAT_Trail
 begin
 
 
@@ -32,8 +32,8 @@ sepref_definition tri_bool_SET_FALSE_impl is "uncurry0 (RETURN 3)" :: "unit_assn
 
 sepref_definition tri_bool_eq_impl is "uncurry (RETURN oo (=))" :: "(unat_assn' TYPE(8))\<^sup>k *\<^sub>a (unat_assn' TYPE(8))\<^sup>k \<rightarrow>\<^sub>a bool1_assn"
   by sepref
-  
-lemmas [sepref_fr_rules] = 
+
+lemmas [sepref_fr_rules] =
   tri_bool_UNSET_impl.refine[FCOMP tri_bool_UNSET_refine_aux]
   tri_bool_SET_TRUE_impl.refine[FCOMP tri_bool_SET_TRUE_refine_aux]
   tri_bool_SET_FALSE_impl.refine[FCOMP tri_bool_SET_FALSE_refine_aux]
@@ -44,13 +44,13 @@ type_synonym trail_pol_fast_assn =
      64 word larray64 \<times> 32 word \<times>
      32 word array_list64\<close>
 
-sepref_definition DECISION_REASON_impl is "uncurry0 (RETURN DECISION_REASON)" 
+sepref_definition DECISION_REASON_impl is "uncurry0 (RETURN DECISION_REASON)"
   :: "unit_assn\<^sup>k \<rightarrow>\<^sub>a sint64_nat_assn"
   unfolding DECISION_REASON_def apply (annot_snat_const "TYPE(64)") by sepref
-lemmas [sepref_fr_rules] = DECISION_REASON_impl.refine  
-     
+lemmas [sepref_fr_rules] = DECISION_REASON_impl.refine
 
-abbreviation trail_pol_fast_assn :: \<open>trail_pol \<Rightarrow> trail_pol_fast_assn \<Rightarrow> assn\<close> where
+
+definition trail_pol_fast_assn :: \<open>trail_pol \<Rightarrow> trail_pol_fast_assn \<Rightarrow> assn\<close> where
   \<open>trail_pol_fast_assn \<equiv>
     arl64_assn unat_lit_assn *a larray64_assn (tri_bool_assn) *a
     larray64_assn uint32_nat_assn *a
@@ -62,100 +62,21 @@ paragraph \<open>Code generation\<close>
 
 subparagraph \<open>Conversion between incomplete and complete mode\<close>
 
-lemma count_decided_pol_workaround: \<open>RETURN o count_decided_pol = (\<lambda>(_, _, _, _, k, _). RETURN k)\<close>
-  unfolding count_decided_pol_def by auto
-  
 
 sepref_definition count_decided_pol_impl is "RETURN o count_decided_pol" :: "trail_pol_fast_assn\<^sup>k \<rightarrow>\<^sub>a uint32_nat_assn"
-  unfolding count_decided_pol_workaround
+  unfolding trail_pol_fast_assn_def count_decided_pol_def
   by sepref
+
 lemmas [sepref_fr_rules] = count_decided_pol_impl.refine
-
-
-(*
-lemma "RETURN
- ((\<lambda>(_::nat literal list, _::bool option list, _::nat list, _::nat list, k::nat,
-      _::nat list). k)
-   (uu::nat literal list \<times> bool option list \<times> nat list \<times> nat list \<times> nat \<times> nat list)) \<equiv>
-RETURN $
-(case_prod $
- (\<lambda>_::nat literal list.
-     PROTECT2
-      (case_prod $
-       (\<lambda>_::bool option list.
-           PROTECT2
-            (case_prod $
-             (\<lambda>_::nat list.
-                 PROTECT2
-                  (case_prod $
-                   (\<lambda>_::nat list.
-                       PROTECT2
-                        (case_prod $
-                         (\<lambda>k::nat. PROTECT2 (\<lambda>_::nat list. PROTECT2 k DUMMY) DUMMY))
-                        DUMMY))
-                  DUMMY))
-            DUMMY))
-      DUMMY) $
- uu) 
-"
-
-
-
-sepref_definition count_decided_pol_impl is "RETURN o count_decided_pol" :: "trail_pol_fast_assn\<^sup>k \<rightarrow>\<^sub>a uint32_nat_assn"
-  unfolding count_decided_pol_def
-  apply sepref_dbg_keep
-  apply (rule ID_init)
-  supply [[trace_f_tac_conv]] [[show_types,show_sorts]]
-  apply (tactic \<open>let 
-    val ctxt = @{context} 
-    
-    fun f_tac_conv ctxt f tac ct = let
-      val t = Thm.term_of ct
-      val t' = f t
-      val goal = Logic.mk_equals (t,t')
-      val _ = tracing (Syntax.string_of_term ctxt goal)
-
-      val goal = Thm.cterm_of ctxt goal handle e => raise (@{print} e)
-
-      val thm = Goal.prove_internal ctxt [] goal (K tac)
-    in
-      thm
-    end
-    
-    
-    fun protect_conv ctxt = f_tac_conv ctxt
-      (Id_Op.protect []) 
-      (simp_tac (put_simpset HOL_basic_ss ctxt addsimps @{thms PROTECT2_def APP_def}) 1)
-      
-      (*
-      (((K (print_tac ctxt "FOO")) THEN' simp_tac 
-        (put_simpset HOL_basic_ss ctxt addsimps @{thms PROTECT2_def APP_def})) 1)
-      *)
-    
-    
-  in
-    (CONVERSION Thm.eta_conversion
-    THEN' CONVERSION (
-        Refine_Util.HOL_concl_conv (fn ctxt => (Id_Op.id_a_conv (protect_conv ctxt))) 
-          ctxt
-      )
-
-    ) 1
-    end
-  \<close>)
-  
-  apply sepref_dbg_id_init
-
-*)  
 
 sepref_definition get_level_atm_fast_code [llvm_code]
   is \<open>uncurry (RETURN oo get_level_atm_pol)\<close>
   :: \<open>[get_level_atm_pol_pre]\<^sub>a
   trail_pol_fast_assn\<^sup>k *\<^sub>a uint32_nat_assn\<^sup>k \<rightarrow> uint32_nat_assn\<close>
-  unfolding get_level_atm_pol_def nat_shiftr_div2[symmetric] 
-     get_level_atm_pol_pre_def
-  supply [[eta_contract = false, show_abbrevs=false]]   
-  apply (rewrite at "nth _" eta_expand)   
+  unfolding get_level_atm_pol_def nat_shiftr_div2[symmetric]
+     get_level_atm_pol_pre_def trail_pol_fast_assn_def
+  supply [[eta_contract = false, show_abbrevs=false]]
+  apply (rewrite at "nth _" eta_expand)
   apply (rewrite in "nth _ \<hole>" annot_unat_snat_upcast[where 'l="64"])
   supply [[goals_limit = 1]]
   by sepref
@@ -179,8 +100,8 @@ sepref_definition polarity_pol_fast_code [llvm_code]
   is \<open>uncurry (RETURN oo polarity_pol)\<close>
   :: \<open>[uncurry polarity_pol_pre]\<^sub>a trail_pol_fast_assn\<^sup>k *\<^sub>a unat_lit_assn\<^sup>k \<rightarrow> tri_bool_assn\<close>
   unfolding polarity_pol_def option.case_eq_if polarity_pol_pre_def
+    trail_pol_fast_assn_def
   supply [[goals_limit = 1]]
-  (*apply (rewrite in "nth _ \<hole>" annot_unat_snat_upcast[where 'l="64"])*)
   by sepref
 
 declare polarity_pol_fast_code.refine[sepref_fr_rules]
@@ -189,6 +110,7 @@ sepref_definition isa_length_trail_fast_code [llvm_code]
   is \<open>RETURN o isa_length_trail\<close>
   :: \<open>[\<lambda>_. True]\<^sub>a trail_pol_fast_assn\<^sup>k \<rightarrow> snat_assn' TYPE(64)\<close>
   unfolding isa_length_trail_def isa_length_trail_pre_def length_uint32_nat_def
+    trail_pol_fast_assn_def
   by sepref
 
 declare isa_length_trail_fast_code.refine[sepref_fr_rules]
@@ -200,7 +122,7 @@ sepref_definition cons_trail_Propagated_tr_fast_code
        unat_lit_assn\<^sup>k *\<^sub>a sint64_nat_assn\<^sup>k *\<^sub>a trail_pol_fast_assn\<^sup>d \<rightarrow> trail_pol_fast_assn\<close>
   unfolding cons_trail_Propagated_tr_def cons_trail_Propagated_tr_def
     SET_TRUE_def[symmetric] SET_FALSE_def[symmetric] cons_trail_Propagated_tr_pre_def
-  unfolding ins_idx_upcast64[where i="atm_of _"]  
+  unfolding ins_idx_upcast64[where i="atm_of _"] trail_pol_fast_assn_def
   (*unfolding ins_idx_upcast64  *)
   supply [[goals_limit = 1]]
   supply [simp] = max_snat_def uint32_max_def
@@ -226,15 +148,15 @@ sepref_definition tl_trail_tr_fast_code
   is \<open>RETURN o tl_trailt_tr\<close>
   :: \<open>[tl_trailt_tr_pre]\<^sub>a
         trail_pol_fast_assn\<^sup>d \<rightarrow> trail_pol_fast_assn\<close>
-  supply if_splits[split] option.splits[split] 
+  supply if_splits[split] option.splits[split]
   unfolding tl_trailt_tr_def UNSET_def[symmetric] tl_trailt_tr_pre_def
-  unfolding ins_idx_upcast64[where i="atm_of _"]  
+  unfolding ins_idx_upcast64[where i="atm_of _"] trail_pol_fast_assn_def
   apply (annot_unat_const "TYPE(32)")
   (*apply (rewrite at \<open>_ - one_uint32_nat\<close> fast_minus_def[symmetric])*)
   supply [[goals_limit = 1]]
   by sepref
-  
-  
+
+
 declare tl_trail_tr_fast_code.refine[sepref_fr_rules]
 
 sepref_definition tl_trail_proped_tr_fast_code
@@ -244,7 +166,7 @@ sepref_definition tl_trail_proped_tr_fast_code
   supply if_splits[split] option.splits[split]
   unfolding tl_trail_propedt_tr_def UNSET_def[symmetric]
     tl_trail_propedt_tr_pre_def
-  unfolding ins_idx_upcast64[where i="atm_of _"]  
+  unfolding ins_idx_upcast64[where i="atm_of _"] trail_pol_fast_assn_def
   apply (annot_unat_const "TYPE(32)")
   supply [[goals_limit = 1]]
   by sepref
@@ -254,7 +176,7 @@ declare tl_trail_proped_tr_fast_code.refine[sepref_fr_rules]
 sepref_definition (in -) lit_of_last_trail_fast_code
   is \<open>RETURN o lit_of_last_trail_pol\<close>
   :: \<open>[\<lambda>(M, _). M \<noteq> []]\<^sub>a trail_pol_fast_assn\<^sup>k \<rightarrow> unat_lit_assn\<close>
-  unfolding lit_of_last_trail_pol_def
+  unfolding lit_of_last_trail_pol_def trail_pol_fast_assn_def
   by sepref
 
 declare lit_of_last_trail_fast_code.refine[sepref_fr_rules]
@@ -263,9 +185,9 @@ sepref_definition cons_trail_Decided_tr_fast_code
   is \<open>uncurry (RETURN oo cons_trail_Decided_tr)\<close>
   :: \<open>[cons_trail_Decided_tr_pre]\<^sub>a
        unat_lit_assn\<^sup>k *\<^sub>a trail_pol_fast_assn\<^sup>d \<rightarrow> trail_pol_fast_assn\<close>
-  unfolding cons_trail_Decided_tr_def cons_trail_Decided_tr_def
+  unfolding cons_trail_Decided_tr_def cons_trail_Decided_tr_def trail_pol_fast_assn_def
     SET_TRUE_def[symmetric] SET_FALSE_def[symmetric] cons_trail_Decided_tr_pre_def
-  unfolding ins_idx_upcast64[where i="atm_of _"]  
+  unfolding ins_idx_upcast64[where i="atm_of _"]
   apply (annot_unat_const "TYPE(32)")
   apply (rewrite at "_@[\<hole>]" in "(_,\<hole>)" annot_snat_unat_downcast[where 'l="32"])
   supply [[goals_limit = 1]]
@@ -278,11 +200,11 @@ sepref_definition defined_atm_fast_code
   is \<open>uncurry (RETURN oo defined_atm_pol)\<close>
   :: \<open>[uncurry defined_atm_pol_pre]\<^sub>a trail_pol_fast_assn\<^sup>k *\<^sub>a uint32_nat_assn\<^sup>k \<rightarrow> bool1_assn\<close>
   unfolding defined_atm_pol_def UNSET_def[symmetric] tri_bool_eq_def[symmetric]
-    defined_atm_pol_pre_def
-  unfolding ins_idx_upcast64  
+    defined_atm_pol_pre_def trail_pol_fast_assn_def
+  unfolding ins_idx_upcast64
   supply [simp] = max_unat_def uint32_max_def max_snat_def
   apply (annot_unat_const "TYPE(32)")
-  supply UNSET_def[simp del] 
+  supply UNSET_def[simp del]
   by sepref
 
 declare defined_atm_fast_code.refine[sepref_fr_rules]
@@ -291,7 +213,7 @@ sepref_register get_propagation_reason_raw_pol
 sepref_definition get_propagation_reason_fast_code
   is \<open>uncurry get_propagation_reason_raw_pol\<close>
   :: \<open>trail_pol_fast_assn\<^sup>k *\<^sub>a unat_lit_assn\<^sup>k \<rightarrow>\<^sub>a sint64_nat_assn\<close>
-  unfolding get_propagation_reason_raw_pol_def
+  unfolding get_propagation_reason_raw_pol_def trail_pol_fast_assn_def
   apply (rewrite at "_! \<hole>" annot_unat_snat_upcast[where 'l="64"])
   by sepref
 
@@ -307,7 +229,7 @@ sepref_definition get_propagation_reason_fast_code
 
 declare get_propagation_reason_fast_code.refine[sepref_fr_rules]
   get_propagation_reason_code.refine[sepref_fr_rules]
-  
+
 
 sepref_definition get_the_propagation_reason_code
   is \<open>uncurry get_the_propagation_reason_pol\<close>
@@ -330,8 +252,8 @@ declare get_the_propagation_reason_fast_code.refine[sepref_fr_rules]
 sepref_definition isa_trail_nth_fast_code
   is \<open>uncurry isa_trail_nth\<close>
   :: \<open>trail_pol_fast_assn\<^sup>k *\<^sub>a uint32_nat_assn\<^sup>k \<rightarrow>\<^sub>a unat_lit_assn\<close>
-  unfolding isa_trail_nth_def
-  unfolding ins_idx_upcast64  
+  unfolding isa_trail_nth_def trail_pol_fast_assn_def
+  unfolding ins_idx_upcast64
   by sepref
 
 declare isa_trail_nth_fast_code.refine[sepref_fr_rules]
@@ -342,14 +264,14 @@ sepref_definition tl_trail_tr_no_CS_fast_code
         trail_pol_fast_assn\<^sup>d \<rightarrow> trail_pol_fast_assn\<close>
   supply if_splits[split] option.splits[split]
   unfolding tl_trailt_tr_no_CS_def UNSET_def[symmetric] tl_trailt_tr_no_CS_pre_def
-  unfolding ins_idx_upcast64[where i="atm_of _"]  
+  unfolding ins_idx_upcast64[where i="atm_of _"] trail_pol_fast_assn_def
   apply (annot_unat_const "TYPE(32)")
   supply [[goals_limit = 1]]
   by sepref
 
-declare tl_trail_tr_no_CS_fast_code.refine[sepref_fr_rules]  
-  
-abbreviation (in -) trail_pol_fast_assn' :: \<open>trail_pol \<Rightarrow> trail_pol_fast_assn \<Rightarrow> assn\<close> where
+declare tl_trail_tr_no_CS_fast_code.refine[sepref_fr_rules]
+
+definition (in -) trail_pol_fast_assn' :: \<open>trail_pol \<Rightarrow> trail_pol_fast_assn \<Rightarrow> assn\<close> where
   \<open>trail_pol_fast_assn' \<equiv>
       arl64_assn unat_lit_assn *a larray64_assn (tri_bool_assn) *a
       larray64_assn uint32_nat_assn *a
@@ -359,10 +281,10 @@ sepref_definition (in -) trail_conv_back_imp_fast_code
   is \<open>uncurry trail_conv_back_imp\<close>
   :: \<open>uint32_nat_assn\<^sup>k *\<^sub>a trail_pol_fast_assn'\<^sup>d \<rightarrow>\<^sub>a trail_pol_fast_assn'\<close>
   supply [[goals_limit=1]]
-  unfolding trail_conv_back_imp_def 
+  unfolding trail_conv_back_imp_def trail_pol_fast_assn'_def
   apply (rewrite at "take \<hole>" annot_unat_snat_upcast[where 'l=64])
   by sepref_dbg_keep
-  
+
 
 declare trail_conv_back_imp_fast_code.refine[sepref_fr_rules]
 
